tests/AddDelay.bpl
@@ -202,8 +202,8 @@ procedure Net#init#6()
   assume 0 == 0;
   M[Net#b][C[Net#b]] := 0;
   C[Net#b] := C[Net#b] + 1;
-  assert {:msg "26.15: Initialization of network 'Net' might not establish the channel invariant (#18)"} M[Net#b][0] == 0;
-  assert {:msg "27.15: Initialization of network 'Net' might not establish the channel invariant (#19)"} 0 <= M[Net#b][I[Net#b]];
+  assert {:msg "24.15: Initialization of network 'Net' might not establish the channel invariant (#18)"} M[Net#b][0] == 0;
+  assert {:msg "25.15: Initialization of network 'Net' might not establish the channel invariant (#19)"} 0 <= M[Net#b][I[Net#b]];
   assert {:msg "Initialization of network 'Net' might not establish the channel invariant (#20)"} I[Net#c] == I[Net#a];
   assert {:msg "Initialization of network 'Net' might not establish the channel invariant (#21)"} I[Net#c] == I[Net#b];
   assert {:msg "Initialization of network 'Net' might not establish the channel invariant (#22)"} I[Net#b] == I[Net#e];
@@ -211,14 +211,10 @@ procedure Net#init#6()
   assert {:msg "Initialization of network 'Net' might not establish the channel invariant (#24)"} I[Net#e] == I[Net#c];
   I := R;
   assert {:msg "23.13: Initialization of network 'Net' might not establish the network invariant (#25)"} (C[Net#b] - R[Net#b]) == 1;
-  assert {:msg "24.13: Initialization of network 'Net' might not establish the network invariant (#26)"} R[Net#a] == C[Net#d];
-  assert {:msg "25.14: Initialization of network 'Net' might not establish the network invariant (#27)"} (forall i: int :: 
-    ((0 + 1) <= i) && (i < (C[Net#d] - 0)) ==> (M[Net#d][i] == (M[Net#d][i - 1] + M[Net#a][i]))
-  );
-  assert {:msg "Initialization of network 'Net' might not establish the network invariant: Unread tokens might be left on channel a (#28)"} (C[Net#a] - R[Net#a]) == 0;
-  assert {:msg "Initialization of network 'Net' might not establish the network invariant: Unread tokens might be left on channel c (#29)"} (C[Net#c] - R[Net#c]) == 0;
-  assert {:msg "Initialization of network 'Net' might not establish the network invariant: Unread tokens might be left on channel d (#30)"} (C[Net#d] - R[Net#d]) == 0;
-  assert {:msg "Initialization of network 'Net' might not establish the network invariant: Unread tokens might be left on channel e (#31)"} (C[Net#e] - R[Net#e]) == 0;
+  assert {:msg "Initialization of network 'Net' might not establish the network invariant: Unread tokens might be left on channel a (#26)"} (C[Net#a] - R[Net#a]) == 0;
+  assert {:msg "Initialization of network 'Net' might not establish the network invariant: Unread tokens might be left on channel c (#27)"} (C[Net#c] - R[Net#c]) == 0;
+  assert {:msg "Initialization of network 'Net' might not establish the network invariant: Unread tokens might be left on channel d (#28)"} (C[Net#d] - R[Net#d]) == 0;
+  assert {:msg "Initialization of network 'Net' might not establish the network invariant: Unread tokens might be left on channel e (#29)"} (C[Net#e] - R[Net#e]) == 0;
 }
 procedure Net##Add#anon$0#7()
   modifies C, R, M, I;
@@ -300,13 +296,13 @@ procedure Net##Add#anon$0#7()
   assume (forall idx$: int :: 
     (0 <= idx$) && (idx$ < C[Net#e]) ==> (M[Net#e][idx$] == M[Net#c][idx$])
   );
-  assert {:msg "26.15: Action at 2.3 ('anon$0') for actor instance 'add' might not preserve the channel invariant (#32)"} M[Net#b][0] == 0;
-  assert {:msg "27.15: Action at 2.3 ('anon$0') for actor instance 'add' might not preserve the channel invariant (#33)"} 0 <= M[Net#b][I[Net#b]];
-  assert {:msg "Action at 2.3 ('anon$0') for actor instance 'add' might not preserve the channel invariant (#34)"} I[Net#c] == I[Net#a];
-  assert {:msg "Action at 2.3 ('anon$0') for actor instance 'add' might not preserve the channel invariant (#35)"} I[Net#c] == I[Net#b];
-  assert {:msg "Action at 2.3 ('anon$0') for actor instance 'add' might not preserve the channel invariant (#36)"} I[Net#b] == I[Net#e];
-  assert {:msg "Action at 2.3 ('anon$0') for actor instance 'add' might not preserve the channel invariant (#37)"} I[Net#d] == I[Net#c];
-  assert {:msg "Action at 2.3 ('anon$0') for actor instance 'add' might not preserve the channel invariant (#38)"} I[Net#e] == I[Net#c];
+  assert {:msg "24.15: Action at 2.3 ('anon$0') for actor instance 'add' might not preserve the channel invariant (#30)"} M[Net#b][0] == 0;
+  assert {:msg "25.15: Action at 2.3 ('anon$0') for actor instance 'add' might not preserve the channel invariant (#31)"} 0 <= M[Net#b][I[Net#b]];
+  assert {:msg "Action at 2.3 ('anon$0') for actor instance 'add' might not preserve the channel invariant (#32)"} I[Net#c] == I[Net#a];
+  assert {:msg "Action at 2.3 ('anon$0') for actor instance 'add' might not preserve the channel invariant (#33)"} I[Net#c] == I[Net#b];
+  assert {:msg "Action at 2.3 ('anon$0') for actor instance 'add' might not preserve the channel invariant (#34)"} I[Net#b] == I[Net#e];
+  assert {:msg "Action at 2.3 ('anon$0') for actor instance 'add' might not preserve the channel invariant (#35)"} I[Net#d] == I[Net#c];
+  assert {:msg "Action at 2.3 ('anon$0') for actor instance 'add' might not preserve the channel invariant (#36)"} I[Net#e] == I[Net#c];
 }
 procedure Net##Delay#anon$3#8()
   modifies C, R, M, I;
@@ -385,13 +381,13 @@ procedure Net##Delay#anon$3#8()
   assume (forall idx$: int :: 
     (0 <= idx$) && (idx$ < C[Net#e]) ==> (M[Net#e][idx$] == M[Net#c][idx$])
   );
-  assert {:msg "26.15: Action at 11.3 ('anon$3') for actor instance 'del' might not preserve the channel invariant (#39)"} M[Net#b][0] == 0;
-  assert {:msg "27.15: Action at 11.3 ('anon$3') for actor instance 'del' might not preserve the channel invariant (#40)"} 0 <= M[Net#b][I[Net#b]];
-  assert {:msg "Action at 11.3 ('anon$3') for actor instance 'del' might not preserve the channel invariant (#41)"} I[Net#c] == I[Net#a];
-  assert {:msg "Action at 11.3 ('anon$3') for actor instance 'del' might not preserve the channel invariant (#42)"} I[Net#c] == I[Net#b];
-  assert {:msg "Action at 11.3 ('anon$3') for actor instance 'del' might not preserve the channel invariant (#43)"} I[Net#b] == I[Net#e];
-  assert {:msg "Action at 11.3 ('anon$3') for actor instance 'del' might not preserve the channel invariant (#44)"} I[Net#d] == I[Net#c];
-  assert {:msg "Action at 11.3 ('anon$3') for actor instance 'del' might not preserve the channel invariant (#45)"} I[Net#e] == I[Net#c];
+  assert {:msg "24.15: Action at 11.3 ('anon$3') for actor instance 'del' might not preserve the channel invariant (#37)"} M[Net#b][0] == 0;
+  assert {:msg "25.15: Action at 11.3 ('anon$3') for actor instance 'del' might not preserve the channel invariant (#38)"} 0 <= M[Net#b][I[Net#b]];
+  assert {:msg "Action at 11.3 ('anon$3') for actor instance 'del' might not preserve the channel invariant (#39)"} I[Net#c] == I[Net#a];
+  assert {:msg "Action at 11.3 ('anon$3') for actor instance 'del' might not preserve the channel invariant (#40)"} I[Net#c] == I[Net#b];
+  assert {:msg "Action at 11.3 ('anon$3') for actor instance 'del' might not preserve the channel invariant (#41)"} I[Net#b] == I[Net#e];
+  assert {:msg "Action at 11.3 ('anon$3') for actor instance 'del' might not preserve the channel invariant (#42)"} I[Net#d] == I[Net#c];
+  assert {:msg "Action at 11.3 ('anon$3') for actor instance 'del' might not preserve the channel invariant (#43)"} I[Net#e] == I[Net#c];
 }
 procedure Net##Split#anon$1#9()
   modifies C, R, M, I;
@@ -472,13 +468,13 @@ procedure Net##Split#anon$1#9()
   assume (forall idx$: int :: 
     (0 <= idx$) && (idx$ < C[Net#e]) ==> (M[Net#e][idx$] == M[Net#c][idx$])
   );
-  assert {:msg "26.15: Action at 6.3 ('anon$1') for actor instance 'spl' might not preserve the channel invariant (#46)"} M[Net#b][0] == 0;
-  assert {:msg "27.15: Action at 6.3 ('anon$1') for actor instance 'spl' might not preserve the channel invariant (#47)"} 0 <= M[Net#b][I[Net#b]];
-  assert {:msg "Action at 6.3 ('anon$1') for actor instance 'spl' might not preserve the channel invariant (#48)"} I[Net#c] == I[Net#a];
-  assert {:msg "Action at 6.3 ('anon$1') for actor instance 'spl' might not preserve the channel invariant (#49)"} I[Net#c] == I[Net#b];
-  assert {:msg "Action at 6.3 ('anon$1') for actor instance 'spl' might not preserve the channel invariant (#50)"} I[Net#b] == I[Net#e];
-  assert {:msg "Action at 6.3 ('anon$1') for actor instance 'spl' might not preserve the channel invariant (#51)"} I[Net#d] == I[Net#c];
-  assert {:msg "Action at 6.3 ('anon$1') for actor instance 'spl' might not preserve the channel invariant (#52)"} I[Net#e] == I[Net#c];
+  assert {:msg "24.15: Action at 6.3 ('anon$1') for actor instance 'spl' might not preserve the channel invariant (#44)"} M[Net#b][0] == 0;
+  assert {:msg "25.15: Action at 6.3 ('anon$1') for actor instance 'spl' might not preserve the channel invariant (#45)"} 0 <= M[Net#b][I[Net#b]];
+  assert {:msg "Action at 6.3 ('anon$1') for actor instance 'spl' might not preserve the channel invariant (#46)"} I[Net#c] == I[Net#a];
+  assert {:msg "Action at 6.3 ('anon$1') for actor instance 'spl' might not preserve the channel invariant (#47)"} I[Net#c] == I[Net#b];
+  assert {:msg "Action at 6.3 ('anon$1') for actor instance 'spl' might not preserve the channel invariant (#48)"} I[Net#b] == I[Net#e];
+  assert {:msg "Action at 6.3 ('anon$1') for actor instance 'spl' might not preserve the channel invariant (#49)"} I[Net#d] == I[Net#c];
+  assert {:msg "Action at 6.3 ('anon$1') for actor instance 'spl' might not preserve the channel invariant (#50)"} I[Net#e] == I[Net#c];
 }
 procedure Net#anon$4#input#in#10()
   modifies C, R, M, I;
@@ -537,14 +533,14 @@ procedure Net#anon$4#input#in#10()
   );
   C[Net#a] := C[Net#a] + 1;
   assume 0 <= M[Net#a][I[Net#a]];
-  assert {:msg "26.15: Channel invariant might be falsified by network input (#53)"} M[Net#b][0] == 0;
-  assert {:msg "27.15: Channel invariant might be falsified by network input (#54)"} 0 <= M[Net#b][I[Net#b]];
-  assert {:msg "Channel invariant might be falsified by network input (#55)"} I[Net#c] == I[Net#a];
-  assert {:msg "Channel invariant might be falsified by network input (#56)"} I[Net#c] == I[Net#b];
-  assert {:msg "Channel invariant might be falsified by network input (#57)"} I[Net#b] == I[Net#e];
-  assert {:msg "Channel invariant might be falsified by network input (#58)"} I[Net#d] == I[Net#c];
-  assert {:msg "Channel invariant might be falsified by network input (#59)"} I[Net#e] == I[Net#c];
-  assert {:msg "17.14: Channel invariant might be falsified by network input (#60)"} 0 <= M[Net#a][I[Net#a]];
+  assert {:msg "24.15: Channel invariant might be falsified by network input (#51)"} M[Net#b][0] == 0;
+  assert {:msg "25.15: Channel invariant might be falsified by network input (#52)"} 0 <= M[Net#b][I[Net#b]];
+  assert {:msg "Channel invariant might be falsified by network input (#53)"} I[Net#c] == I[Net#a];
+  assert {:msg "Channel invariant might be falsified by network input (#54)"} I[Net#c] == I[Net#b];
+  assert {:msg "Channel invariant might be falsified by network input (#55)"} I[Net#b] == I[Net#e];
+  assert {:msg "Channel invariant might be falsified by network input (#56)"} I[Net#d] == I[Net#c];
+  assert {:msg "Channel invariant might be falsified by network input (#57)"} I[Net#e] == I[Net#c];
+  assert {:msg "17.14: Channel invariant might be falsified by network input (#58)"} 0 <= M[Net#a][I[Net#a]];
 }
 procedure Net#anon$4#exit#11()
   modifies C, R, M, I;
@@ -605,25 +601,21 @@ procedure Net#anon$4#exit#11()
   assume !((1 <= (C[Net#a] - R[Net#a])) && (1 <= (C[Net#b] - R[Net#b])));
   assume !(1 <= (C[Net#e] - R[Net#e]));
   assume !(1 <= (C[Net#c] - R[Net#c]));
-  assert {:msg "18.13: Network action postcondition might not hold (#61)"} M[Net#d][0] == M[Net#a][0];
-  assert {:msg "19.13: Network action postcondition might not hold (#62)"} M[Net#d][I[Net#d]] >= M[Net#a][I[Net#a]];
-  assert {:msg "20.13: Network action postcondition might not hold (#63)"} (0 < I[Net#d]) ==> (M[Net#d][I[Net#d]] == (M[Net#d][I[Net#d] - 1] + M[Net#a][I[Net#a]]));
+  assert {:msg "18.13: Network action postcondition might not hold (#59)"} M[Net#d][0] == M[Net#a][0];
+  assert {:msg "19.13: Network action postcondition might not hold (#60)"} M[Net#d][I[Net#d]] >= M[Net#a][I[Net#a]];
+  assert {:msg "20.13: Network action postcondition might not hold (#61)"} (0 < I[Net#d]) ==> (M[Net#d][I[Net#d]] == (M[Net#d][I[Net#d] - 1] + M[Net#a][I[Net#a]]));
   R[Net#d] := R[Net#d] + 1;
   I := R;
-  assert {:msg "26.15: The network might not preserve the channel invariant (#64)"} M[Net#b][0] == 0;
-  assert {:msg "27.15: The network might not preserve the channel invariant (#65)"} 0 <= M[Net#b][I[Net#b]];
-  assert {:msg "The network might not preserve the channel invariant (#66)"} I[Net#c] == I[Net#a];
-  assert {:msg "The network might not preserve the channel invariant (#67)"} I[Net#c] == I[Net#b];
-  assert {:msg "The network might not preserve the channel invariant (#68)"} I[Net#b] == I[Net#e];
-  assert {:msg "The network might not preserve the channel invariant (#69)"} I[Net#d] == I[Net#c];
-  assert {:msg "The network might not preserve the channel invariant (#70)"} I[Net#e] == I[Net#c];
-  assert {:msg "23.13: The network might not preserve the network invariant (#71)"} (C[Net#b] - R[Net#b]) == 1;
-  assert {:msg "24.13: The network might not preserve the network invariant (#72)"} R[Net#a] == C[Net#d];
-  assert {:msg "25.14: The network might not preserve the network invariant (#73)"} (forall i: int :: 
-    ((0 + 1) <= i) && (i < (C[Net#d] - 0)) ==> (M[Net#d][i] == (M[Net#d][i - 1] + M[Net#a][i]))
-  );
-  assert {:msg "The network might not preserve the network invariant: Unread tokens might be left on channel a (#74)"} (C[Net#a] - R[Net#a]) == 0;
-  assert {:msg "The network might not preserve the network invariant: Unread tokens might be left on channel c (#75)"} (C[Net#c] - R[Net#c]) == 0;
-  assert {:msg "The network might not preserve the network invariant: Unread tokens might be left on channel d (#76)"} (C[Net#d] - R[Net#d]) == 0;
-  assert {:msg "The network might not preserve the network invariant: Unread tokens might be left on channel e (#77)"} (C[Net#e] - R[Net#e]) == 0;
+  assert {:msg "24.15: The network might not preserve the channel invariant (#62)"} M[Net#b][0] == 0;
+  assert {:msg "25.15: The network might not preserve the channel invariant (#63)"} 0 <= M[Net#b][I[Net#b]];
+  assert {:msg "The network might not preserve the channel invariant (#64)"} I[Net#c] == I[Net#a];
+  assert {:msg "The network might not preserve the channel invariant (#65)"} I[Net#c] == I[Net#b];
+  assert {:msg "The network might not preserve the channel invariant (#66)"} I[Net#b] == I[Net#e];
+  assert {:msg "The network might not preserve the channel invariant (#67)"} I[Net#d] == I[Net#c];
+  assert {:msg "The network might not preserve the channel invariant (#68)"} I[Net#e] == I[Net#c];
+  assert {:msg "23.13: The network might not preserve the network invariant (#69)"} (C[Net#b] - R[Net#b]) == 1;
+  assert {:msg "The network might not preserve the network invariant: Unread tokens might be left on channel a (#70)"} (C[Net#a] - R[Net#a]) == 0;
+  assert {:msg "The network might not preserve the network invariant: Unread tokens might be left on channel c (#71)"} (C[Net#c] - R[Net#c]) == 0;
+  assert {:msg "The network might not preserve the network invariant: Unread tokens might be left on channel d (#72)"} (C[Net#d] - R[Net#d]) == 0;
+  assert {:msg "The network might not preserve the network invariant: Unread tokens might be left on channel e (#73)"} (C[Net#e] - R[Net#e]) == 0;
 }
