tests/DataDependent.bpl
@@ -53,8 +53,8 @@ procedure Gain#anon$0#1()
   R[in] := R[in] + 1;
   M[out][C[out]] := 2 * in#0;
   C[out] := C[out] + 1;
-  assert {:msg "Action at 2.3 might not preserve invariant (#2)"} R[in] == C[out];
-  assert {:msg "Action at 2.3 might not preserve invariant (#3)"} (forall idx$: int :: 
+  assert {:msg "Action at 3.3 might not preserve invariant (#2)"} R[in] == C[out];
+  assert {:msg "Action at 3.3 might not preserve invariant (#3)"} (forall idx$: int :: 
     (0 <= idx$) && (idx$ < C[out]) ==> (M[out][idx$] == (2 * M[in][idx$]))
   );
 }
@@ -68,9 +68,9 @@ procedure Split#init#2()
   assume R[in] == 0;
   assume C[pos] == 0;
   assume C[neg] == 0;
-  assert {:msg "6.13: Initialization might not establish the invariant (#4)"} R[in] == (C[pos] + C[neg]);
-  assert {:msg "7.13: Initialization might not establish the invariant (#5)"} (0 < R[in]) && (0 <= M[in][R[in] - 1]) ==> (M[in][R[in] - 1] == M[pos][C[pos] - 1]);
-  assert {:msg "8.13: Initialization might not establish the invariant (#6)"} (0 < R[in]) && (M[in][R[in] - 1] < 0) ==> (M[in][R[in] - 1] == M[neg][C[neg] - 1]);
+  assert {:msg "7.20: Initialization might not establish the invariant (#4)"} R[in] == (C[pos] + C[neg]);
+  assert {:msg "8.20: Initialization might not establish the invariant (#5)"} (0 < R[in]) && (0 <= M[in][R[in] - 1]) ==> (M[in][R[in] - 1] == M[pos][C[pos] - 1]);
+  assert {:msg "9.20: Initialization might not establish the invariant (#6)"} (0 < R[in]) && (M[in][R[in] - 1] < 0) ==> (M[in][R[in] - 1] == M[neg][C[neg] - 1]);
 }
 procedure Split#anon$1#3()
   modifies C, R, M, I;
@@ -91,9 +91,9 @@ procedure Split#anon$1#3()
   assume 0 <= in#0;
   M[pos][C[pos]] := in#0;
   C[pos] := C[pos] + 1;
-  assert {:msg "6.13: Action at 9.3 might not preserve invariant (#7)"} R[in] == (C[pos] + C[neg]);
-  assert {:msg "7.13: Action at 9.3 might not preserve invariant (#8)"} (0 < R[in]) && (0 <= M[in][R[in] - 1]) ==> (M[in][R[in] - 1] == M[pos][C[pos] - 1]);
-  assert {:msg "8.13: Action at 9.3 might not preserve invariant (#9)"} (0 < R[in]) && (M[in][R[in] - 1] < 0) ==> (M[in][R[in] - 1] == M[neg][C[neg] - 1]);
+  assert {:msg "7.20: Action at 10.3 might not preserve invariant (#7)"} R[in] == (C[pos] + C[neg]);
+  assert {:msg "8.20: Action at 10.3 might not preserve invariant (#8)"} (0 < R[in]) && (0 <= M[in][R[in] - 1]) ==> (M[in][R[in] - 1] == M[pos][C[pos] - 1]);
+  assert {:msg "9.20: Action at 10.3 might not preserve invariant (#9)"} (0 < R[in]) && (M[in][R[in] - 1] < 0) ==> (M[in][R[in] - 1] == M[neg][C[neg] - 1]);
 }
 procedure Split#anon$2#4()
   modifies C, R, M, I;
@@ -114,9 +114,9 @@ procedure Split#anon$2#4()
   assume in#0 < 0;
   M[neg][C[neg]] := in#0;
   C[neg] := C[neg] + 1;
-  assert {:msg "6.13: Action at 12.3 might not preserve invariant (#10)"} R[in] == (C[pos] + C[neg]);
-  assert {:msg "7.13: Action at 12.3 might not preserve invariant (#11)"} (0 < R[in]) && (0 <= M[in][R[in] - 1]) ==> (M[in][R[in] - 1] == M[pos][C[pos] - 1]);
-  assert {:msg "8.13: Action at 12.3 might not preserve invariant (#12)"} (0 < R[in]) && (M[in][R[in] - 1] < 0) ==> (M[in][R[in] - 1] == M[neg][C[neg] - 1]);
+  assert {:msg "7.20: Action at 13.3 might not preserve invariant (#10)"} R[in] == (C[pos] + C[neg]);
+  assert {:msg "8.20: Action at 13.3 might not preserve invariant (#11)"} (0 < R[in]) && (0 <= M[in][R[in] - 1]) ==> (M[in][R[in] - 1] == M[pos][C[pos] - 1]);
+  assert {:msg "9.20: Action at 13.3 might not preserve invariant (#12)"} (0 < R[in]) && (M[in][R[in] - 1] < 0) ==> (M[in][R[in] - 1] == M[neg][C[neg] - 1]);
 }
 procedure Split##GuardWD#5()
   modifies C, R, M, I;
@@ -126,7 +126,7 @@ procedure Split##GuardWD#5()
   var neg: Chan (int);
   var in#0: int;
   assume (in != pos) && (in != neg) && (pos != neg);
-  assert {:msg "5.1: The actions of actor 'Split' might not have mutually exclusive guards (#13)"} !((1 <= (C[in] - R[in])) && (0 <= in#0) && (1 <= (C[in] - R[in])) && (in#0 < 0));
+  assert {:msg "6.1: The actions of actor 'Split' might not have mutually exclusive guards (#13)"} !((1 <= (C[in] - R[in])) && (0 <= in#0) && (1 <= (C[in] - R[in])) && (in#0 < 0));
 }
 procedure Net#init#6()
   modifies C, R, M, I;
@@ -161,16 +161,16 @@ procedure Net#init#6()
   assume R[Net#c] == 0;
   assume C[Net#d] == 0;
   assume R[Net#d] == 0;
-  assert {:msg "31.15: Initialization of network 'Net' might not establish the channel invariant (#14)"} I[Net#b] == (I[Net#d] + I[Net#c]);
-  assert {:msg "33.15: Initialization of network 'Net' might not establish the channel invariant (#15)"} (0 < C[Net#a]) ==> ((M[Net#a][I[Net#a]] == 1) || (M[Net#a][I[Net#a]] == (-1)));
-  assert {:msg "34.15: Initialization of network 'Net' might not establish the channel invariant (#16)"} (0 < R[Net#b]) && (M[Net#b][I[Net#b]] >= 0) ==> (C[Net#d] == 0);
-  assert {:msg "35.15: Initialization of network 'Net' might not establish the channel invariant (#17)"} (0 < R[Net#b]) && (M[Net#b][I[Net#b]] < 0) ==> (C[Net#c] == 0);
+  assert {:msg "32.15: Initialization of network 'Net' might not establish the channel invariant (#14)"} I[Net#b] == (I[Net#d] + I[Net#c]);
+  assert {:msg "33.15: Initialization of network 'Net' might not establish the channel invariant (#15)"} (0 < (C[Net#a] - I[Net#a])) ==> ((M[Net#a][I[Net#a]] == 1) || (M[Net#a][I[Net#a]] == (-1)));
+  assert {:msg "34.15: Initialization of network 'Net' might not establish the channel invariant (#16)"} (0 < (R[Net#b] - I[Net#b])) && (M[Net#b][I[Net#b]] >= 0) ==> ((C[Net#d] - I[Net#d]) == 0);
+  assert {:msg "35.15: Initialization of network 'Net' might not establish the channel invariant (#17)"} (0 < (R[Net#b] - I[Net#b])) && (M[Net#b][I[Net#b]] < 0) ==> ((C[Net#c] - I[Net#c]) == 0);
   assert {:msg "Initialization of network 'Net' might not establish the channel invariant (#18)"} I[Net#b] == I[Net#a];
   I := R;
-  assert {:msg "43.5: The initialization might produce unspecified tokens on channel a (#19)"} (C[Net#a] - R[Net#a]) == 0;
-  assert {:msg "44.5: The initialization might produce unspecified tokens on channel b (#20)"} (C[Net#b] - R[Net#b]) == 0;
-  assert {:msg "45.5: The initialization might produce unspecified tokens on channel c (#21)"} (C[Net#c] - R[Net#c]) == 0;
-  assert {:msg "46.5: The initialization might produce unspecified tokens on channel d (#22)"} (C[Net#d] - R[Net#d]) == 0;
+  assert {:msg "Initialization of network 'Net' might not establish the network invariant: Unread tokens might be left on channel a (#19)"} (C[Net#a] - R[Net#a]) == 0;
+  assert {:msg "Initialization of network 'Net' might not establish the network invariant: Unread tokens might be left on channel b (#20)"} (C[Net#b] - R[Net#b]) == 0;
+  assert {:msg "Initialization of network 'Net' might not establish the network invariant: Unread tokens might be left on channel c (#21)"} (C[Net#c] - R[Net#c]) == 0;
+  assert {:msg "Initialization of network 'Net' might not establish the network invariant: Unread tokens might be left on channel d (#22)"} (C[Net#d] - R[Net#d]) == 0;
 }
 procedure Net##Gain#anon$0#7()
   modifies C, R, M, I;
@@ -199,9 +199,9 @@ procedure Net##Gain#anon$0#7()
   assume R[Net#d] <= C[Net#d];
   assume I[Net#d] == R[Net#d];
   assume I[Net#b] == (I[Net#d] + I[Net#c]);
-  assume (0 < C[Net#a]) ==> ((M[Net#a][I[Net#a]] == 1) || (M[Net#a][I[Net#a]] == (-1)));
-  assume (0 < R[Net#b]) && (M[Net#b][I[Net#b]] >= 0) ==> (C[Net#d] == 0);
-  assume (0 < R[Net#b]) && (M[Net#b][I[Net#b]] < 0) ==> (C[Net#c] == 0);
+  assume (0 < (C[Net#a] - I[Net#a])) ==> ((M[Net#a][I[Net#a]] == 1) || (M[Net#a][I[Net#a]] == (-1)));
+  assume (0 < (R[Net#b] - I[Net#b])) && (M[Net#b][I[Net#b]] >= 0) ==> ((C[Net#d] - I[Net#d]) == 0);
+  assume (0 < (R[Net#b] - I[Net#b])) && (M[Net#b][I[Net#b]] < 0) ==> ((C[Net#c] - I[Net#c]) == 0);
   assume I[Net#b] == I[Net#a];
   assume ((M[Net#a][I[Net#a]] == 1) && (forall i: int :: 
     (I[Net#a] <= i) && (i < C[Net#a]) ==> (M[Net#a][i] == 1)
@@ -212,6 +212,9 @@ procedure Net##Gain#anon$0#7()
   assume (forall idx$: int :: 
     (0 <= idx$) && (idx$ < C[Net#b]) ==> (M[Net#b][idx$] == (2 * M[Net#a][idx$]))
   );
+  assume R[Net#b] == (C[Net#c] + C[Net#d]);
+  assume (0 < R[Net#b]) && (0 <= M[Net#b][R[Net#b] - 1]) ==> (M[Net#b][R[Net#b] - 1] == M[Net#c][C[Net#c] - 1]);
+  assume (0 < R[Net#b]) && (M[Net#b][R[Net#b] - 1] < 0) ==> (M[Net#b][R[Net#b] - 1] == M[Net#d][C[Net#d] - 1]);
   assume 1 <= (C[Net#a] - R[Net#a]);
   in#i := M[Net#a][R[Net#a]];
   R[Net#a] := R[Net#a] + 1;
@@ -221,11 +224,14 @@ procedure Net##Gain#anon$0#7()
   assume (forall idx$: int :: 
     (0 <= idx$) && (idx$ < C[Net#b]) ==> (M[Net#b][idx$] == (2 * M[Net#a][idx$]))
   );
-  assert {:msg "31.15: Action at 2.3 ('anon$0') for actor instance 'gain' might not preserve the channel invariant (#23)"} I[Net#b] == (I[Net#d] + I[Net#c]);
-  assert {:msg "33.15: Action at 2.3 ('anon$0') for actor instance 'gain' might not preserve the channel invariant (#24)"} (0 < C[Net#a]) ==> ((M[Net#a][I[Net#a]] == 1) || (M[Net#a][I[Net#a]] == (-1)));
-  assert {:msg "34.15: Action at 2.3 ('anon$0') for actor instance 'gain' might not preserve the channel invariant (#25)"} (0 < R[Net#b]) && (M[Net#b][I[Net#b]] >= 0) ==> (C[Net#d] == 0);
-  assert {:msg "35.15: Action at 2.3 ('anon$0') for actor instance 'gain' might not preserve the channel invariant (#26)"} (0 < R[Net#b]) && (M[Net#b][I[Net#b]] < 0) ==> (C[Net#c] == 0);
-  assert {:msg "Action at 2.3 ('anon$0') for actor instance 'gain' might not preserve the channel invariant (#27)"} I[Net#b] == I[Net#a];
+  assume R[Net#b] == (C[Net#c] + C[Net#d]);
+  assume (0 < R[Net#b]) && (0 <= M[Net#b][R[Net#b] - 1]) ==> (M[Net#b][R[Net#b] - 1] == M[Net#c][C[Net#c] - 1]);
+  assume (0 < R[Net#b]) && (M[Net#b][R[Net#b] - 1] < 0) ==> (M[Net#b][R[Net#b] - 1] == M[Net#d][C[Net#d] - 1]);
+  assert {:msg "32.15: Action at 3.3 ('anon$0') for actor instance 'gain' might not preserve the channel invariant (#23)"} I[Net#b] == (I[Net#d] + I[Net#c]);
+  assert {:msg "33.15: Action at 3.3 ('anon$0') for actor instance 'gain' might not preserve the channel invariant (#24)"} (0 < (C[Net#a] - I[Net#a])) ==> ((M[Net#a][I[Net#a]] == 1) || (M[Net#a][I[Net#a]] == (-1)));
+  assert {:msg "34.15: Action at 3.3 ('anon$0') for actor instance 'gain' might not preserve the channel invariant (#25)"} (0 < (R[Net#b] - I[Net#b])) && (M[Net#b][I[Net#b]] >= 0) ==> ((C[Net#d] - I[Net#d]) == 0);
+  assert {:msg "35.15: Action at 3.3 ('anon$0') for actor instance 'gain' might not preserve the channel invariant (#26)"} (0 < (R[Net#b] - I[Net#b])) && (M[Net#b][I[Net#b]] < 0) ==> ((C[Net#c] - I[Net#c]) == 0);
+  assert {:msg "Action at 3.3 ('anon$0') for actor instance 'gain' might not preserve the channel invariant (#27)"} I[Net#b] == I[Net#a];
 }
 procedure Net##Split#anon$1#8()
   modifies C, R, M, I;
@@ -254,9 +260,9 @@ procedure Net##Split#anon$1#8()
   assume R[Net#d] <= C[Net#d];
   assume I[Net#d] == R[Net#d];
   assume I[Net#b] == (I[Net#d] + I[Net#c]);
-  assume (0 < C[Net#a]) ==> ((M[Net#a][I[Net#a]] == 1) || (M[Net#a][I[Net#a]] == (-1)));
-  assume (0 < R[Net#b]) && (M[Net#b][I[Net#b]] >= 0) ==> (C[Net#d] == 0);
-  assume (0 < R[Net#b]) && (M[Net#b][I[Net#b]] < 0) ==> (C[Net#c] == 0);
+  assume (0 < (C[Net#a] - I[Net#a])) ==> ((M[Net#a][I[Net#a]] == 1) || (M[Net#a][I[Net#a]] == (-1)));
+  assume (0 < (R[Net#b] - I[Net#b])) && (M[Net#b][I[Net#b]] >= 0) ==> ((C[Net#d] - I[Net#d]) == 0);
+  assume (0 < (R[Net#b] - I[Net#b])) && (M[Net#b][I[Net#b]] < 0) ==> ((C[Net#c] - I[Net#c]) == 0);
   assume I[Net#b] == I[Net#a];
   assume ((M[Net#a][I[Net#a]] == 1) && (forall i: int :: 
     (I[Net#a] <= i) && (i < C[Net#a]) ==> (M[Net#a][i] == 1)
@@ -267,6 +273,9 @@ procedure Net##Split#anon$1#8()
   assume (forall idx$: int :: 
     (0 <= idx$) && (idx$ < C[Net#b]) ==> (M[Net#b][idx$] == (2 * M[Net#a][idx$]))
   );
+  assume R[Net#b] == (C[Net#c] + C[Net#d]);
+  assume (0 < R[Net#b]) && (0 <= M[Net#b][R[Net#b] - 1]) ==> (M[Net#b][R[Net#b] - 1] == M[Net#c][C[Net#c] - 1]);
+  assume (0 < R[Net#b]) && (M[Net#b][R[Net#b] - 1] < 0) ==> (M[Net#b][R[Net#b] - 1] == M[Net#d][C[Net#d] - 1]);
   assume (1 <= (C[Net#b] - R[Net#b])) && (0 <= M[Net#b][R[Net#b]]);
   in#i := M[Net#b][R[Net#b]];
   R[Net#b] := R[Net#b] + 1;
@@ -276,11 +285,14 @@ procedure Net##Split#anon$1#8()
   assume (forall idx$: int :: 
     (0 <= idx$) && (idx$ < C[Net#b]) ==> (M[Net#b][idx$] == (2 * M[Net#a][idx$]))
   );
-  assert {:msg "31.15: Action at 9.3 ('anon$1') for actor instance 'split' might not preserve the channel invariant (#28)"} I[Net#b] == (I[Net#d] + I[Net#c]);
-  assert {:msg "33.15: Action at 9.3 ('anon$1') for actor instance 'split' might not preserve the channel invariant (#29)"} (0 < C[Net#a]) ==> ((M[Net#a][I[Net#a]] == 1) || (M[Net#a][I[Net#a]] == (-1)));
-  assert {:msg "34.15: Action at 9.3 ('anon$1') for actor instance 'split' might not preserve the channel invariant (#30)"} (0 < R[Net#b]) && (M[Net#b][I[Net#b]] >= 0) ==> (C[Net#d] == 0);
-  assert {:msg "35.15: Action at 9.3 ('anon$1') for actor instance 'split' might not preserve the channel invariant (#31)"} (0 < R[Net#b]) && (M[Net#b][I[Net#b]] < 0) ==> (C[Net#c] == 0);
-  assert {:msg "Action at 9.3 ('anon$1') for actor instance 'split' might not preserve the channel invariant (#32)"} I[Net#b] == I[Net#a];
+  assume R[Net#b] == (C[Net#c] + C[Net#d]);
+  assume (0 < R[Net#b]) && (0 <= M[Net#b][R[Net#b] - 1]) ==> (M[Net#b][R[Net#b] - 1] == M[Net#c][C[Net#c] - 1]);
+  assume (0 < R[Net#b]) && (M[Net#b][R[Net#b] - 1] < 0) ==> (M[Net#b][R[Net#b] - 1] == M[Net#d][C[Net#d] - 1]);
+  assert {:msg "32.15: Action at 10.3 ('anon$1') for actor instance 'split' might not preserve the channel invariant (#28)"} I[Net#b] == (I[Net#d] + I[Net#c]);
+  assert {:msg "33.15: Action at 10.3 ('anon$1') for actor instance 'split' might not preserve the channel invariant (#29)"} (0 < (C[Net#a] - I[Net#a])) ==> ((M[Net#a][I[Net#a]] == 1) || (M[Net#a][I[Net#a]] == (-1)));
+  assert {:msg "34.15: Action at 10.3 ('anon$1') for actor instance 'split' might not preserve the channel invariant (#30)"} (0 < (R[Net#b] - I[Net#b])) && (M[Net#b][I[Net#b]] >= 0) ==> ((C[Net#d] - I[Net#d]) == 0);
+  assert {:msg "35.15: Action at 10.3 ('anon$1') for actor instance 'split' might not preserve the channel invariant (#31)"} (0 < (R[Net#b] - I[Net#b])) && (M[Net#b][I[Net#b]] < 0) ==> ((C[Net#c] - I[Net#c]) == 0);
+  assert {:msg "Action at 10.3 ('anon$1') for actor instance 'split' might not preserve the channel invariant (#32)"} I[Net#b] == I[Net#a];
 }
 procedure Net##Split#anon$2#9()
   modifies C, R, M, I;
@@ -309,9 +321,9 @@ procedure Net##Split#anon$2#9()
   assume R[Net#d] <= C[Net#d];
   assume I[Net#d] == R[Net#d];
   assume I[Net#b] == (I[Net#d] + I[Net#c]);
-  assume (0 < C[Net#a]) ==> ((M[Net#a][I[Net#a]] == 1) || (M[Net#a][I[Net#a]] == (-1)));
-  assume (0 < R[Net#b]) && (M[Net#b][I[Net#b]] >= 0) ==> (C[Net#d] == 0);
-  assume (0 < R[Net#b]) && (M[Net#b][I[Net#b]] < 0) ==> (C[Net#c] == 0);
+  assume (0 < (C[Net#a] - I[Net#a])) ==> ((M[Net#a][I[Net#a]] == 1) || (M[Net#a][I[Net#a]] == (-1)));
+  assume (0 < (R[Net#b] - I[Net#b])) && (M[Net#b][I[Net#b]] >= 0) ==> ((C[Net#d] - I[Net#d]) == 0);
+  assume (0 < (R[Net#b] - I[Net#b])) && (M[Net#b][I[Net#b]] < 0) ==> ((C[Net#c] - I[Net#c]) == 0);
   assume I[Net#b] == I[Net#a];
   assume ((M[Net#a][I[Net#a]] == 1) && (forall i: int :: 
     (I[Net#a] <= i) && (i < C[Net#a]) ==> (M[Net#a][i] == 1)
@@ -322,6 +334,9 @@ procedure Net##Split#anon$2#9()
   assume (forall idx$: int :: 
     (0 <= idx$) && (idx$ < C[Net#b]) ==> (M[Net#b][idx$] == (2 * M[Net#a][idx$]))
   );
+  assume R[Net#b] == (C[Net#c] + C[Net#d]);
+  assume (0 < R[Net#b]) && (0 <= M[Net#b][R[Net#b] - 1]) ==> (M[Net#b][R[Net#b] - 1] == M[Net#c][C[Net#c] - 1]);
+  assume (0 < R[Net#b]) && (M[Net#b][R[Net#b] - 1] < 0) ==> (M[Net#b][R[Net#b] - 1] == M[Net#d][C[Net#d] - 1]);
   assume (1 <= (C[Net#b] - R[Net#b])) && (M[Net#b][R[Net#b]] < 0);
   in#j := M[Net#b][R[Net#b]];
   R[Net#b] := R[Net#b] + 1;
@@ -331,11 +346,14 @@ procedure Net##Split#anon$2#9()
   assume (forall idx$: int :: 
     (0 <= idx$) && (idx$ < C[Net#b]) ==> (M[Net#b][idx$] == (2 * M[Net#a][idx$]))
   );
-  assert {:msg "31.15: Action at 12.3 ('anon$2') for actor instance 'split' might not preserve the channel invariant (#33)"} I[Net#b] == (I[Net#d] + I[Net#c]);
-  assert {:msg "33.15: Action at 12.3 ('anon$2') for actor instance 'split' might not preserve the channel invariant (#34)"} (0 < C[Net#a]) ==> ((M[Net#a][I[Net#a]] == 1) || (M[Net#a][I[Net#a]] == (-1)));
-  assert {:msg "34.15: Action at 12.3 ('anon$2') for actor instance 'split' might not preserve the channel invariant (#35)"} (0 < R[Net#b]) && (M[Net#b][I[Net#b]] >= 0) ==> (C[Net#d] == 0);
-  assert {:msg "35.15: Action at 12.3 ('anon$2') for actor instance 'split' might not preserve the channel invariant (#36)"} (0 < R[Net#b]) && (M[Net#b][I[Net#b]] < 0) ==> (C[Net#c] == 0);
-  assert {:msg "Action at 12.3 ('anon$2') for actor instance 'split' might not preserve the channel invariant (#37)"} I[Net#b] == I[Net#a];
+  assume R[Net#b] == (C[Net#c] + C[Net#d]);
+  assume (0 < R[Net#b]) && (0 <= M[Net#b][R[Net#b] - 1]) ==> (M[Net#b][R[Net#b] - 1] == M[Net#c][C[Net#c] - 1]);
+  assume (0 < R[Net#b]) && (M[Net#b][R[Net#b] - 1] < 0) ==> (M[Net#b][R[Net#b] - 1] == M[Net#d][C[Net#d] - 1]);
+  assert {:msg "32.15: Action at 13.3 ('anon$2') for actor instance 'split' might not preserve the channel invariant (#33)"} I[Net#b] == (I[Net#d] + I[Net#c]);
+  assert {:msg "33.15: Action at 13.3 ('anon$2') for actor instance 'split' might not preserve the channel invariant (#34)"} (0 < (C[Net#a] - I[Net#a])) ==> ((M[Net#a][I[Net#a]] == 1) || (M[Net#a][I[Net#a]] == (-1)));
+  assert {:msg "34.15: Action at 13.3 ('anon$2') for actor instance 'split' might not preserve the channel invariant (#35)"} (0 < (R[Net#b] - I[Net#b])) && (M[Net#b][I[Net#b]] >= 0) ==> ((C[Net#d] - I[Net#d]) == 0);
+  assert {:msg "35.15: Action at 13.3 ('anon$2') for actor instance 'split' might not preserve the channel invariant (#36)"} (0 < (R[Net#b] - I[Net#b])) && (M[Net#b][I[Net#b]] < 0) ==> ((C[Net#c] - I[Net#c]) == 0);
+  assert {:msg "Action at 13.3 ('anon$2') for actor instance 'split' might not preserve the channel invariant (#37)"} I[Net#b] == I[Net#a];
 }
 procedure Net#anon$3#input#in#10()
   modifies C, R, M, I;
@@ -364,9 +382,9 @@ procedure Net#anon$3#input#in#10()
   assume I[Net#d] == R[Net#d];
   assume (C[Net#a] - I[Net#a]) < 1;
   assume I[Net#b] == (I[Net#d] + I[Net#c]);
-  assume (0 < C[Net#a]) ==> ((M[Net#a][I[Net#a]] == 1) || (M[Net#a][I[Net#a]] == (-1)));
-  assume (0 < R[Net#b]) && (M[Net#b][I[Net#b]] >= 0) ==> (C[Net#d] == 0);
-  assume (0 < R[Net#b]) && (M[Net#b][I[Net#b]] < 0) ==> (C[Net#c] == 0);
+  assume (0 < (C[Net#a] - I[Net#a])) ==> ((M[Net#a][I[Net#a]] == 1) || (M[Net#a][I[Net#a]] == (-1)));
+  assume (0 < (R[Net#b] - I[Net#b])) && (M[Net#b][I[Net#b]] >= 0) ==> ((C[Net#d] - I[Net#d]) == 0);
+  assume (0 < (R[Net#b] - I[Net#b])) && (M[Net#b][I[Net#b]] < 0) ==> ((C[Net#c] - I[Net#c]) == 0);
   assume I[Net#b] == I[Net#a];
   assume ((M[Net#a][I[Net#a]] == 1) && (forall i: int :: 
     (I[Net#a] <= i) && (i < C[Net#a]) ==> (M[Net#a][i] == 1)
@@ -377,15 +395,18 @@ procedure Net#anon$3#input#in#10()
   assume (forall idx$: int :: 
     (0 <= idx$) && (idx$ < C[Net#b]) ==> (M[Net#b][idx$] == (2 * M[Net#a][idx$]))
   );
+  assume R[Net#b] == (C[Net#c] + C[Net#d]);
+  assume (0 < R[Net#b]) && (0 <= M[Net#b][R[Net#b] - 1]) ==> (M[Net#b][R[Net#b] - 1] == M[Net#c][C[Net#c] - 1]);
+  assume (0 < R[Net#b]) && (M[Net#b][R[Net#b] - 1] < 0) ==> (M[Net#b][R[Net#b] - 1] == M[Net#d][C[Net#d] - 1]);
   C[Net#a] := C[Net#a] + 1;
   assume M[Net#a][I[Net#a]] == 1;
   assume (forall i: int :: 
     (I[Net#a] <= i) && (i < C[Net#a]) ==> (M[Net#a][i] == 1)
   );
-  assert {:msg "31.15: Channel invariant might be falsified by network input (#38)"} I[Net#b] == (I[Net#d] + I[Net#c]);
-  assert {:msg "33.15: Channel invariant might be falsified by network input (#39)"} (0 < C[Net#a]) ==> ((M[Net#a][I[Net#a]] == 1) || (M[Net#a][I[Net#a]] == (-1)));
-  assert {:msg "34.15: Channel invariant might be falsified by network input (#40)"} (0 < R[Net#b]) && (M[Net#b][I[Net#b]] >= 0) ==> (C[Net#d] == 0);
-  assert {:msg "35.15: Channel invariant might be falsified by network input (#41)"} (0 < R[Net#b]) && (M[Net#b][I[Net#b]] < 0) ==> (C[Net#c] == 0);
+  assert {:msg "32.15: Channel invariant might be falsified by network input (#38)"} I[Net#b] == (I[Net#d] + I[Net#c]);
+  assert {:msg "33.15: Channel invariant might be falsified by network input (#39)"} (0 < (C[Net#a] - I[Net#a])) ==> ((M[Net#a][I[Net#a]] == 1) || (M[Net#a][I[Net#a]] == (-1)));
+  assert {:msg "34.15: Channel invariant might be falsified by network input (#40)"} (0 < (R[Net#b] - I[Net#b])) && (M[Net#b][I[Net#b]] >= 0) ==> ((C[Net#d] - I[Net#d]) == 0);
+  assert {:msg "35.15: Channel invariant might be falsified by network input (#41)"} (0 < (R[Net#b] - I[Net#b])) && (M[Net#b][I[Net#b]] < 0) ==> ((C[Net#c] - I[Net#c]) == 0);
   assert {:msg "Channel invariant might be falsified by network input (#42)"} I[Net#b] == I[Net#a];
   assert {:msg "Channel invariant might be falsified by network input (#43)"} ((M[Net#a][I[Net#a]] == 1) && (forall i: int :: 
     (I[Net#a] <= i) && (i < C[Net#a]) ==> (M[Net#a][i] == 1)
@@ -419,9 +440,9 @@ procedure Net#anon$3#exit#11()
   assume R[Net#d] <= C[Net#d];
   assume I[Net#d] == R[Net#d];
   assume I[Net#b] == (I[Net#d] + I[Net#c]);
-  assume (0 < C[Net#a]) ==> ((M[Net#a][I[Net#a]] == 1) || (M[Net#a][I[Net#a]] == (-1)));
-  assume (0 < R[Net#b]) && (M[Net#b][I[Net#b]] >= 0) ==> (C[Net#d] == 0);
-  assume (0 < R[Net#b]) && (M[Net#b][I[Net#b]] < 0) ==> (C[Net#c] == 0);
+  assume (0 < (C[Net#a] - I[Net#a])) ==> ((M[Net#a][I[Net#a]] == 1) || (M[Net#a][I[Net#a]] == (-1)));
+  assume (0 < (R[Net#b] - I[Net#b])) && (M[Net#b][I[Net#b]] >= 0) ==> ((C[Net#d] - I[Net#d]) == 0);
+  assume (0 < (R[Net#b] - I[Net#b])) && (M[Net#b][I[Net#b]] < 0) ==> ((C[Net#c] - I[Net#c]) == 0);
   assume I[Net#b] == I[Net#a];
   assume ((M[Net#a][I[Net#a]] == 1) && (forall i: int :: 
     (I[Net#a] <= i) && (i < C[Net#a]) ==> (M[Net#a][i] == 1)
@@ -432,6 +453,9 @@ procedure Net#anon$3#exit#11()
   assume (forall idx$: int :: 
     (0 <= idx$) && (idx$ < C[Net#b]) ==> (M[Net#b][idx$] == (2 * M[Net#a][idx$]))
   );
+  assume R[Net#b] == (C[Net#c] + C[Net#d]);
+  assume (0 < R[Net#b]) && (0 <= M[Net#b][R[Net#b] - 1]) ==> (M[Net#b][R[Net#b] - 1] == M[Net#c][C[Net#c] - 1]);
+  assume (0 < R[Net#b]) && (M[Net#b][R[Net#b] - 1] < 0) ==> (M[Net#b][R[Net#b] - 1] == M[Net#d][C[Net#d] - 1]);
   assume (C[Net#a] - I[Net#a]) == 1;
   assume M[Net#a][I[Net#a]] == 1;
   assume (forall i: int :: 
@@ -440,19 +464,19 @@ procedure Net#anon$3#exit#11()
   assume !(1 <= (C[Net#a] - R[Net#a]));
   assume !((1 <= (C[Net#b] - R[Net#b])) && (0 <= M[Net#b][R[Net#b]]));
   assume !((1 <= (C[Net#b] - R[Net#b])) && (M[Net#b][R[Net#b]] < 0));
-  assert {:msg "22.13: Network action postcondition might not hold (#44)"} M[Net#c][I[Net#c]] == (2 * M[Net#a][I[Net#a]]);
+  assert {:msg "23.13: Network action postcondition might not hold (#44)"} M[Net#c][I[Net#c]] == (2 * M[Net#a][I[Net#a]]);
   R[Net#c] := R[Net#c] + 1;
   R[Net#d] := R[Net#d] + 0;
   I := R;
-  assert {:msg "31.15: The network might not preserve the channel invariant (#45)"} I[Net#b] == (I[Net#d] + I[Net#c]);
-  assert {:msg "33.15: The network might not preserve the channel invariant (#46)"} (0 < C[Net#a]) ==> ((M[Net#a][I[Net#a]] == 1) || (M[Net#a][I[Net#a]] == (-1)));
-  assert {:msg "34.15: The network might not preserve the channel invariant (#47)"} (0 < R[Net#b]) && (M[Net#b][I[Net#b]] >= 0) ==> (C[Net#d] == 0);
-  assert {:msg "35.15: The network might not preserve the channel invariant (#48)"} (0 < R[Net#b]) && (M[Net#b][I[Net#b]] < 0) ==> (C[Net#c] == 0);
+  assert {:msg "32.15: The network might not preserve the channel invariant (#45)"} I[Net#b] == (I[Net#d] + I[Net#c]);
+  assert {:msg "33.15: The network might not preserve the channel invariant (#46)"} (0 < (C[Net#a] - I[Net#a])) ==> ((M[Net#a][I[Net#a]] == 1) || (M[Net#a][I[Net#a]] == (-1)));
+  assert {:msg "34.15: The network might not preserve the channel invariant (#47)"} (0 < (R[Net#b] - I[Net#b])) && (M[Net#b][I[Net#b]] >= 0) ==> ((C[Net#d] - I[Net#d]) == 0);
+  assert {:msg "35.15: The network might not preserve the channel invariant (#48)"} (0 < (R[Net#b] - I[Net#b])) && (M[Net#b][I[Net#b]] < 0) ==> ((C[Net#c] - I[Net#c]) == 0);
   assert {:msg "The network might not preserve the channel invariant (#49)"} I[Net#b] == I[Net#a];
-  assert {:msg "19.3: The network might leave unread tokens on channel a (#50)"} (C[Net#a] - R[Net#a]) == 0;
-  assert {:msg "19.3: The network might leave unread tokens on channel b (#51)"} (C[Net#b] - R[Net#b]) == 0;
-  assert {:msg "19.3: The network might not produce the specified number of tokens on output out1 (#52)"} (C[Net#c] - R[Net#c]) == 0;
-  assert {:msg "19.3: The network might not produce the specified number of tokens on output out2 (#53)"} (C[Net#d] - R[Net#d]) == 0;
+  assert {:msg "The network might not preserve the network invariant: Unread tokens might be left on channel a (#50)"} (C[Net#a] - R[Net#a]) == 0;
+  assert {:msg "The network might not preserve the network invariant: Unread tokens might be left on channel b (#51)"} (C[Net#b] - R[Net#b]) == 0;
+  assert {:msg "The network might not preserve the network invariant: Unread tokens might be left on channel c (#52)"} (C[Net#c] - R[Net#c]) == 0;
+  assert {:msg "The network might not preserve the network invariant: Unread tokens might be left on channel d (#53)"} (C[Net#d] - R[Net#d]) == 0;
 }
 procedure Net#anon$4#input#in#12()
   modifies C, R, M, I;
@@ -481,9 +505,9 @@ procedure Net#anon$4#input#in#12()
   assume I[Net#d] == R[Net#d];
   assume (C[Net#a] - I[Net#a]) < 1;
   assume I[Net#b] == (I[Net#d] + I[Net#c]);
-  assume (0 < C[Net#a]) ==> ((M[Net#a][I[Net#a]] == 1) || (M[Net#a][I[Net#a]] == (-1)));
-  assume (0 < R[Net#b]) && (M[Net#b][I[Net#b]] >= 0) ==> (C[Net#d] == 0);
-  assume (0 < R[Net#b]) && (M[Net#b][I[Net#b]] < 0) ==> (C[Net#c] == 0);
+  assume (0 < (C[Net#a] - I[Net#a])) ==> ((M[Net#a][I[Net#a]] == 1) || (M[Net#a][I[Net#a]] == (-1)));
+  assume (0 < (R[Net#b] - I[Net#b])) && (M[Net#b][I[Net#b]] >= 0) ==> ((C[Net#d] - I[Net#d]) == 0);
+  assume (0 < (R[Net#b] - I[Net#b])) && (M[Net#b][I[Net#b]] < 0) ==> ((C[Net#c] - I[Net#c]) == 0);
   assume I[Net#b] == I[Net#a];
   assume ((M[Net#a][I[Net#a]] == 1) && (forall i: int :: 
     (I[Net#a] <= i) && (i < C[Net#a]) ==> (M[Net#a][i] == 1)
@@ -494,15 +518,18 @@ procedure Net#anon$4#input#in#12()
   assume (forall idx$: int :: 
     (0 <= idx$) && (idx$ < C[Net#b]) ==> (M[Net#b][idx$] == (2 * M[Net#a][idx$]))
   );
+  assume R[Net#b] == (C[Net#c] + C[Net#d]);
+  assume (0 < R[Net#b]) && (0 <= M[Net#b][R[Net#b] - 1]) ==> (M[Net#b][R[Net#b] - 1] == M[Net#c][C[Net#c] - 1]);
+  assume (0 < R[Net#b]) && (M[Net#b][R[Net#b] - 1] < 0) ==> (M[Net#b][R[Net#b] - 1] == M[Net#d][C[Net#d] - 1]);
   C[Net#a] := C[Net#a] + 1;
   assume M[Net#a][I[Net#a]] == (-1);
   assume (forall i: int :: 
     (I[Net#a] <= i) && (i < C[Net#a]) ==> (M[Net#a][i] == (-1))
   );
-  assert {:msg "31.15: Channel invariant might be falsified by network input (#54)"} I[Net#b] == (I[Net#d] + I[Net#c]);
-  assert {:msg "33.15: Channel invariant might be falsified by network input (#55)"} (0 < C[Net#a]) ==> ((M[Net#a][I[Net#a]] == 1) || (M[Net#a][I[Net#a]] == (-1)));
-  assert {:msg "34.15: Channel invariant might be falsified by network input (#56)"} (0 < R[Net#b]) && (M[Net#b][I[Net#b]] >= 0) ==> (C[Net#d] == 0);
-  assert {:msg "35.15: Channel invariant might be falsified by network input (#57)"} (0 < R[Net#b]) && (M[Net#b][I[Net#b]] < 0) ==> (C[Net#c] == 0);
+  assert {:msg "32.15: Channel invariant might be falsified by network input (#54)"} I[Net#b] == (I[Net#d] + I[Net#c]);
+  assert {:msg "33.15: Channel invariant might be falsified by network input (#55)"} (0 < (C[Net#a] - I[Net#a])) ==> ((M[Net#a][I[Net#a]] == 1) || (M[Net#a][I[Net#a]] == (-1)));
+  assert {:msg "34.15: Channel invariant might be falsified by network input (#56)"} (0 < (R[Net#b] - I[Net#b])) && (M[Net#b][I[Net#b]] >= 0) ==> ((C[Net#d] - I[Net#d]) == 0);
+  assert {:msg "35.15: Channel invariant might be falsified by network input (#57)"} (0 < (R[Net#b] - I[Net#b])) && (M[Net#b][I[Net#b]] < 0) ==> ((C[Net#c] - I[Net#c]) == 0);
   assert {:msg "Channel invariant might be falsified by network input (#58)"} I[Net#b] == I[Net#a];
   assert {:msg "Channel invariant might be falsified by network input (#59)"} ((M[Net#a][I[Net#a]] == 1) && (forall i: int :: 
     (I[Net#a] <= i) && (i < C[Net#a]) ==> (M[Net#a][i] == 1)
@@ -536,9 +563,9 @@ procedure Net#anon$4#exit#13()
   assume R[Net#d] <= C[Net#d];
   assume I[Net#d] == R[Net#d];
   assume I[Net#b] == (I[Net#d] + I[Net#c]);
-  assume (0 < C[Net#a]) ==> ((M[Net#a][I[Net#a]] == 1) || (M[Net#a][I[Net#a]] == (-1)));
-  assume (0 < R[Net#b]) && (M[Net#b][I[Net#b]] >= 0) ==> (C[Net#d] == 0);
-  assume (0 < R[Net#b]) && (M[Net#b][I[Net#b]] < 0) ==> (C[Net#c] == 0);
+  assume (0 < (C[Net#a] - I[Net#a])) ==> ((M[Net#a][I[Net#a]] == 1) || (M[Net#a][I[Net#a]] == (-1)));
+  assume (0 < (R[Net#b] - I[Net#b])) && (M[Net#b][I[Net#b]] >= 0) ==> ((C[Net#d] - I[Net#d]) == 0);
+  assume (0 < (R[Net#b] - I[Net#b])) && (M[Net#b][I[Net#b]] < 0) ==> ((C[Net#c] - I[Net#c]) == 0);
   assume I[Net#b] == I[Net#a];
   assume ((M[Net#a][I[Net#a]] == 1) && (forall i: int :: 
     (I[Net#a] <= i) && (i < C[Net#a]) ==> (M[Net#a][i] == 1)
@@ -549,6 +576,9 @@ procedure Net#anon$4#exit#13()
   assume (forall idx$: int :: 
     (0 <= idx$) && (idx$ < C[Net#b]) ==> (M[Net#b][idx$] == (2 * M[Net#a][idx$]))
   );
+  assume R[Net#b] == (C[Net#c] + C[Net#d]);
+  assume (0 < R[Net#b]) && (0 <= M[Net#b][R[Net#b] - 1]) ==> (M[Net#b][R[Net#b] - 1] == M[Net#c][C[Net#c] - 1]);
+  assume (0 < R[Net#b]) && (M[Net#b][R[Net#b] - 1] < 0) ==> (M[Net#b][R[Net#b] - 1] == M[Net#d][C[Net#d] - 1]);
   assume (C[Net#a] - I[Net#a]) == 1;
   assume M[Net#a][I[Net#a]] == (-1);
   assume (forall i: int :: 
@@ -557,17 +587,17 @@ procedure Net#anon$4#exit#13()
   assume !(1 <= (C[Net#a] - R[Net#a]));
   assume !((1 <= (C[Net#b] - R[Net#b])) && (0 <= M[Net#b][R[Net#b]]));
   assume !((1 <= (C[Net#b] - R[Net#b])) && (M[Net#b][R[Net#b]] < 0));
-  assert {:msg "28.13: Network action postcondition might not hold (#60)"} M[Net#d][I[Net#d]] == (2 * M[Net#a][I[Net#a]]);
+  assert {:msg "29.13: Network action postcondition might not hold (#60)"} M[Net#d][I[Net#d]] == (2 * M[Net#a][I[Net#a]]);
   R[Net#c] := R[Net#c] + 0;
   R[Net#d] := R[Net#d] + 1;
   I := R;
-  assert {:msg "31.15: The network might not preserve the channel invariant (#61)"} I[Net#b] == (I[Net#d] + I[Net#c]);
-  assert {:msg "33.15: The network might not preserve the channel invariant (#62)"} (0 < C[Net#a]) ==> ((M[Net#a][I[Net#a]] == 1) || (M[Net#a][I[Net#a]] == (-1)));
-  assert {:msg "34.15: The network might not preserve the channel invariant (#63)"} (0 < R[Net#b]) && (M[Net#b][I[Net#b]] >= 0) ==> (C[Net#d] == 0);
-  assert {:msg "35.15: The network might not preserve the channel invariant (#64)"} (0 < R[Net#b]) && (M[Net#b][I[Net#b]] < 0) ==> (C[Net#c] == 0);
+  assert {:msg "32.15: The network might not preserve the channel invariant (#61)"} I[Net#b] == (I[Net#d] + I[Net#c]);
+  assert {:msg "33.15: The network might not preserve the channel invariant (#62)"} (0 < (C[Net#a] - I[Net#a])) ==> ((M[Net#a][I[Net#a]] == 1) || (M[Net#a][I[Net#a]] == (-1)));
+  assert {:msg "34.15: The network might not preserve the channel invariant (#63)"} (0 < (R[Net#b] - I[Net#b])) && (M[Net#b][I[Net#b]] >= 0) ==> ((C[Net#d] - I[Net#d]) == 0);
+  assert {:msg "35.15: The network might not preserve the channel invariant (#64)"} (0 < (R[Net#b] - I[Net#b])) && (M[Net#b][I[Net#b]] < 0) ==> ((C[Net#c] - I[Net#c]) == 0);
   assert {:msg "The network might not preserve the channel invariant (#65)"} I[Net#b] == I[Net#a];
-  assert {:msg "25.3: The network might leave unread tokens on channel a (#66)"} (C[Net#a] - R[Net#a]) == 0;
-  assert {:msg "25.3: The network might leave unread tokens on channel b (#67)"} (C[Net#b] - R[Net#b]) == 0;
-  assert {:msg "25.3: The network might not produce the specified number of tokens on output out1 (#68)"} (C[Net#c] - R[Net#c]) == 0;
-  assert {:msg "25.3: The network might not produce the specified number of tokens on output out2 (#69)"} (C[Net#d] - R[Net#d]) == 0;
+  assert {:msg "The network might not preserve the network invariant: Unread tokens might be left on channel a (#66)"} (C[Net#a] - R[Net#a]) == 0;
+  assert {:msg "The network might not preserve the network invariant: Unread tokens might be left on channel b (#67)"} (C[Net#b] - R[Net#b]) == 0;
+  assert {:msg "The network might not preserve the network invariant: Unread tokens might be left on channel c (#68)"} (C[Net#c] - R[Net#c]) == 0;
+  assert {:msg "The network might not preserve the network invariant: Unread tokens might be left on channel d (#69)"} (C[Net#d] - R[Net#d]) == 0;
 }
